commit before making Func.Run well-defined

Blanc/NewCommon.lean
@@ -5,10 +5,6 @@
 import Mathlib.Tactic.Have
 import Blanc.NewSemantics
 
-structure Exec' : Type where
-  (evm : Evm)
-  (exn : Execution)
-  (ex : Exec evm exn)
 
 def compsize : Func → Nat
   | .last _ => 1
@@ -70,11 +66,287 @@ def subcode (cd : B8L) (k : Nat) : Option B8L → Prop
   | none => False
   | some bs => List.Slice cd k bs
 
+/-----------------------------------------------------
+
+structure Pack : Type where
+  (evm : Evm)
+  (evm' : Evm)
+  (ex : Exec evm (.ok evm'))
+
+abbrev Pack.Pred : Type := Pack → Prop
+
+def Pack.imp (π π' : Pack.Pred) : Pack.Pred := λ pk => π pk → π' pk
+
+infix:70 " →p " => Pack.imp
+
+def Pack.Fa (π : Pack.Pred) : Prop := ∀ pk, π pk
+
+notation "□p" => Pack.Fa
+
+inductive Pack.Rel : Pack → Pack → Prop
+  | none {evm : Evm} {n : Ninst} {evm' evm'' : Evm}
+    (n_at : n.At evm.code evm.pc)
+    (run : Ninst.Run' evm n .none (.ok evm'))
+    (ex : Exec evm' (.ok evm'')) :
+    Pack.Rel ⟨evm', evm'', ex⟩ ⟨evm, evm'', .nextNoneRec n_at run ex ⟩
+  | fst {evm : Evm} {n : Ninst} {revm revm' : Evm} {evm' evm'' : Evm}
+    (n_at : n.At evm.code evm.pc)
+    (run : Ninst.Run' evm n (.some (revm, .ok revm')) (.ok evm'))
+    (rex : Exec revm (.ok revm')) (ex : Exec evm' (.ok evm'')) :
+    Pack.Rel ⟨revm, revm', rex⟩ ⟨evm, evm'', .nextSomeRec n_at run rex ex⟩
+  | snd {evm : Evm} {n : Ninst} {revm : Evm}
+    {rexn : Execution} {evm' evm'' : Evm}
+    (n_at : n.At evm.code evm.pc)
+    (run : Ninst.Run' evm n (.some (revm, rexn)) (.ok evm'))
+    (rex : Exec revm rexn) (ex : Exec evm' (.ok evm'')) :
+    Pack.Rel ⟨evm', evm'', ex⟩ ⟨evm, evm'', .nextSomeRec n_at run rex ex⟩
+  | jump {evm : Evm} {j : Jinst} {evm' evm'' : Evm}
+    (j_at : j.At evm.code evm.pc)
+    (run : Jinst.Run' evm j (.ok evm'))
+    (ex : Exec evm' (.ok evm'')) :
+    Pack.Rel ⟨evm', evm'', ex⟩ ⟨evm, evm'', .jumpRec j_at run ex⟩
+
+inductive Pack.le : Pack → Pack → Prop
+  | refl : ∀ p, Pack.le p p
+  | step : ∀ p p' p'', Pack.le p p' → Pack.Rel p' p'' → Pack.le p p''
+
+inductive Pack.lt : Pack → Pack → Prop
+  | intro {pk pk' pk'' : Pack} :
+    Pack.le pk pk' → Pack.Rel pk' pk'' → Pack.lt pk pk''
+
+lemma Pack.lt_of_prec {pk pk' : Pack} (rel : Rel pk pk') : lt pk pk' :=
+  .intro (le.refl pk) rel
+
+def Pack.gt (pk pk' : Pack) : Prop := Pack.lt pk' pk
+
+lemma Pack.eq_or_lt_of_le :
+  ∀ {p p'}, Pack.le p p' → p = p' ∨ Pack.lt p p' := by
+  intros p p'' h0
+  rcases h0 with ⟨_, _, p'⟩ | ⟨p', _, h1, h2⟩
+  · left; rfl
+  · right; refine (.intro h1 h2)
+
+lemma Pack.acc_of_le {pk pk' : Pack}
+    (h_le : Pack.le pk pk') (h_acc : Acc Pack.lt pk') : Acc Pack.lt pk := by
+  cases Pack.eq_or_lt_of_le h_le with
+  | inl h => rw [h]; exact h_acc
+  | inr h => exact Acc.inv h_acc h
+
+theorem Pack.lt.well_founded : WellFounded Pack.lt := by
+
+  have foo :=
+    @Exec.rec
+      ( λ evm exn ex =>
+        ∀ (evm' : Evm) (eq : exn = (.ok evm')),
+          let ex' : Exec evm (.ok evm') := by
+            rw [← eq]; exact ex
+          Acc Pack.lt ⟨evm, evm', ex'⟩ )
+      (by intro _ _ _ eq; cases eq)
+      ( by intro _ _ exn _ _ err _ eq;
+           rw [eq] at err
+           simp [Except.IsError] at err )
+      ( by intro _ _ _ _ _ _ _ _ err _ _ eq
+           rw [eq] at err
+           simp [Except.IsError] at err )
+      ( by intro evm n evm' exn n_at run ex ih
+           intro _evm eq _ex
+           cases _ex; clear _ex
+
+
+
+
+
+
+
+
+
+      )
+
+
+
+
+
+      sorry
+      sorry
+      sorry
+      sorry
+
+
+
+  constructor; intro pk; rcases pk with ⟨evm_0, evm_1, ex_0⟩
+  apply @foo evm_0 (.ok evm_1) ex_0 evm_1 rfl
+
+
+
+
+
+
+
+
+
+
+
+
+
+
+
+
+
+  --apply @Exec.rec (λ s r cr => Acc Pack.lt ⟨s, r, cr⟩)
+
+
+
+#exit
+theorem Pack.lt.well_founded : WellFounded Pack.lt := by
+  constructor; intro pk; rcases pk with ⟨_, _, cr⟩
+  apply @Exec.rec (λ s r cr => Acc Pack.lt ⟨s, r, cr⟩)
+  · intro evm get; constructor;
+    intro _ h; rcases h with ⟨_, _, _, ⟨_⟩⟩
+  · intro _ _ _ _ _ _; constructor;
+    intro _ h; rcases h with ⟨_, _, _, ⟨_⟩⟩
+  · intro evm n evm' exn' exn get run ex' err acc;
+    constructor; intro _ lt
+    rcases lt with ⟨le, ⟨_⟩⟩
+    apply Pack.acc_of_le le acc
+  · intro _ _ _ _ _ _ _ _; constructor;
+    intro _ h; rcases h with ⟨_, _, _, ⟨_⟩⟩
+  · intro evm n evm' exn' evm'' exn get run ex' ex acc acc'
+    constructor; intro _ lt; rcases lt with ⟨le, ⟨_⟩⟩
+    · apply Pack.acc_of_le le acc
+    · apply Pack.acc_of_le le acc'
+  · intro _ _ _ _ _ _; constructor
+    intro _ h; rcases h with ⟨_, _, _, ⟨_⟩⟩
+  · intro _ _ _ _ _ _ _ _; constructor
+    intro _ h; rcases h with ⟨_, _, _, ⟨_⟩⟩
+  · intro _ _ _ _ _; constructor
+    intro _ h; rcases h with ⟨_, _, _, ⟨_⟩⟩
+
+def carryover (π : Pack.Pred) : Pack.Pred :=
+(λ pk => □p (Pack.gt pk →p π)) →p π
+
+def Exec'.strongRec (π : Exec'.Pred) : □p (carryover π) → □p π := by
+  intro ih pk
+  apply @WellFounded.induction _ Exec'.lt Exec'.lt.well_founded π pk
+  clear pk; intro pk ih'
+  apply ih
+  intro pk' h_gt
+  apply ih' _ h_gt
+infix:70 " →p " => Exec'.imp
+
+-------------------------------------------------------------------------/
+
+structure Pack : Type where
+  (evm : Evm)
+  (exn : Execution)
+  (ex : Exec evm exn)
+
+abbrev Pack.Pred : Type := Pack → Prop
+
+def Pack.imp (π π' : Pack.Pred) : Pack.Pred := λ pk => π pk → π' pk
+
+infix:70 " →p " => Pack.imp
+
+def Pack.Fa (π : Pack.Pred) : Prop := ∀ pk, π pk
+
+notation "□p" => Pack.Fa
+
+inductive Pack.Rel : Pack → Pack → Prop
+  | none {evm : Evm} {n : Ninst} {evm' : Evm} {exn : Execution}
+    (n_at : n.At evm.code evm.pc)
+    (run : Ninst.Run' evm n .none (.ok evm'))
+    (ex : Exec evm' exn) :
+    Pack.Rel ⟨evm', exn, ex⟩ ⟨evm, exn, .nextNoneRec n_at run ex⟩
+  | fst {evm : Evm} {n : Ninst} {revm : Evm}
+    {rexn : Execution} {evm' evm'' : Evm}
+    (n_at : n.At evm.code evm.pc)
+    (run : Ninst.Run' evm n (.some (revm, rexn)) (.ok evm'))
+    (rex : Exec revm rexn) (ex : Exec evm' (.ok evm'')) :
+    Pack.Rel ⟨revm, rexn, rex⟩ ⟨evm, .ok evm'', .nextSomeRec n_at run rex ex⟩
+  | snd {evm : Evm} {n : Ninst} {revm : Evm}
+    {rexn : Execution} {evm' evm'' : Evm}
+    (n_at : n.At evm.code evm.pc)
+    (run : Ninst.Run' evm n (.some (revm, rexn)) (.ok evm'))
+    (rex : Exec revm rexn) (ex : Exec evm' (.ok evm'')) :
+    Pack.Rel ⟨evm', .ok evm'', ex⟩ ⟨evm, .ok evm'', .nextSomeRec n_at run rex ex⟩
+  | jump {evm : Evm} {j : Jinst} {evm' evm'' : Evm}
+    (j_at : j.At evm.code evm.pc)
+    (run : Jinst.Run' evm j (.ok evm'))
+    (ex : Exec evm' (.ok evm'')) :
+    Pack.Rel ⟨evm', .ok evm'', ex⟩ ⟨evm, .ok evm'', .jumpRec j_at run ex⟩
+
+inductive Pack.le : Pack → Pack → Prop
+  | refl : ∀ p, Pack.le p p
+  | step : ∀ {p p' p''}, Pack.le p p' → Pack.Rel p' p'' → Pack.le p p''
+
+inductive Pack.lt : Pack → Pack → Prop
+  | intro {pk pk' pk'' : Pack} :
+    Pack.le pk pk' → Pack.Rel pk' pk'' → Pack.lt pk pk''
+
+lemma Pack.lt_of_prec {pk pk' : Pack} (rel : Rel pk pk') : lt pk pk' :=
+  .intro (le.refl pk) rel
+
+def Pack.gt (pk pk' : Pack) : Prop := Pack.lt pk' pk
+
+lemma Pack.eq_or_lt_of_le :
+  ∀ {p p'}, Pack.le p p' → p = p' ∨ Pack.lt p p' := by
+  intros p p'' h0
+  rcases h0 with ⟨_, _, _⟩ | ⟨h1, h2⟩
+  · left; rfl
+  · right; refine (.intro h1 h2)
+
+lemma Pack.acc_of_le {pk pk' : Pack}
+    (h_le : Pack.le pk pk') (h_acc : Acc Pack.lt pk') : Acc Pack.lt pk := by
+  cases Pack.eq_or_lt_of_le h_le with
+  | inl h => rw [h]; exact h_acc
+  | inr h => exact Acc.inv h_acc h
+
+theorem Pack.lt.well_founded : WellFounded Pack.lt := by
+  constructor; intro pk; rcases pk with ⟨_, _, cr⟩
+  apply @Exec.rec (λ s r cr => Acc Pack.lt ⟨s, r, cr⟩)
+  · intro evm get; constructor;
+    intro _ h; rcases h with ⟨_, ⟨_⟩⟩
+  · intro _ _ _ _ _ _; constructor;
+    intro _ h; rcases h with ⟨_, ⟨_⟩⟩
+  · intro evm n evm' exn' exn get run ex' err acc;
+    constructor; intro _ lt
+    rcases lt with ⟨le, ⟨_⟩⟩
+  · intro _ _ _ _ _ _ _ acc; constructor;
+    intro _ h; rcases h with ⟨le, ⟨_⟩⟩;
+    apply Pack.acc_of_le le acc
+  · intro evm n evm' exn' evm'' exn get run ex' ex acc acc'
+    constructor; intro _ lt; rcases lt with ⟨le, ⟨_⟩⟩
+    · apply Pack.acc_of_le le acc
+    · apply Pack.acc_of_le le acc'
+  · intro _ _ _ _ _ _; constructor
+    intro _ h; rcases h with ⟨_, ⟨_⟩⟩
+  · intro _ _ _ _ _ _ _ acc; constructor
+    intro _ h; rcases h with ⟨le, ⟨_⟩⟩
+    apply Pack.acc_of_le le acc
+  · intro _ _ _ _ _; constructor
+    intro _ h; rcases h with ⟨_, ⟨_⟩⟩
+
+def carryover (π : Pack.Pred) : Pack.Pred :=
+  (λ pk => □p (Pack.gt pk →p π)) →p π
+
+def Pack.strongRec (π : Pack.Pred) : □p (carryover π) → □p π := by
+  intro ih pk
+  apply @WellFounded.induction _ Pack.lt Pack.lt.well_founded π pk
+  clear pk; intro pk ih'
+  apply ih
+  intro pk' h_gt
+  apply ih' _ h_gt
+
+
+
+/-
+structure Exec' : Type where
+  (evm : Evm)
+  (exn : Execution)
+  (ex : Exec evm exn)
+
 abbrev Exec'.Pred : Type := Exec' → Prop
 
 def Exec'.imp (π π' : Exec'.Pred) : Exec'.Pred := λ pk => π pk → π' pk
-
-infix:70 " →p " => Exec'.imp
 
 def Exec'.Fa (π : Exec'.Pred) : Prop := ∀ pk, π pk
 
@@ -105,11 +377,11 @@ inductive Exec'.le : Exec' → Exec' → Prop
   | step : ∀ p p' p'', Exec'.le p p' → Exec'.Rel p' p'' → Exec'.le p p''
 
 inductive Exec'.lt : Exec' → Exec' → Prop
-  | intro (pk pk' pk'' : Exec') :
+  | intro {pk pk' pk'' : Exec'} :
     Exec'.le pk pk' → Exec'.Rel pk' pk'' → Exec'.lt pk pk''
 
 lemma Exec'.lt_of_prec {pk pk' : Exec'} (rel : Rel pk pk') : lt pk pk' :=
-  .intro _ _ _ (le.refl pk) rel
+  .intro (le.refl pk) rel
 
 def Exec'.gt (pk pk' : Exec') : Prop := Exec'.lt pk' pk
 
@@ -118,7 +390,7 @@ lemma Exec'.eq_or_lt_of_le :
   intros p p'' h0
   rcases h0 with ⟨_, _, p'⟩ | ⟨p', _, h1, h2⟩
   · left; rfl
-  · right; refine (.intro _ _ _ h1 h2)
+  · right; refine (.intro h1 h2)
 
 lemma Exec'.acc_of_le {pk pk' : Exec'}
     (h_le : Exec'.le pk pk') (h_acc : Acc Exec'.lt pk') : Acc Exec'.lt pk := by
@@ -135,12 +407,12 @@ theorem Exec'.lt.well_founded : WellFounded Exec'.lt := by
     intro _ h; rcases h with ⟨_, _, _, ⟨_⟩⟩
   · intro evm n evm' exn' exn get run ex' err acc;
     constructor; intro _ lt
-    rcases lt with ⟨_, _ , le, ⟨_⟩⟩
+    rcases lt with ⟨le, ⟨_⟩⟩
     apply Exec'.acc_of_le le acc
   · intro _ _ _ _ _ _ _ _; constructor;
     intro _ h; rcases h with ⟨_, _, _, ⟨_⟩⟩
   · intro evm n evm' exn' evm'' exn get run ex' ex acc acc'
-    constructor; intro _ lt; rcases lt with ⟨_, _ , le, ⟨_⟩⟩
+    constructor; intro _ lt; rcases lt with ⟨le, ⟨_⟩⟩
     · apply Exec'.acc_of_le le acc
     · apply Exec'.acc_of_le le acc'
   · intro _ _ _ _ _ _; constructor
@@ -160,6 +432,7 @@ def Exec'.strongRec (π : Exec'.Pred) : □p (carryover π) → □p π := by
   apply ih
   intro pk' h_gt
   apply ih' _ h_gt
+-/
 
 lemma Linst.run_of_at {evm l exn} (ex : Exec evm exn)
     (get : l.At evm.code evm.pc) : Linst.Run' evm l exn := by
@@ -258,18 +531,15 @@ lemma toB8_toRinst {i : Rinst} : B8.toRinst i.toB8 = some i := by
   · apply swap_toByte_toRinst?
   · apply log_toByte_toRinst?
 
+lemma Linst.toRinst_toB8_eq_none {l : Linst} : l.toB8.toRinst = .none := by cases l <;> rfl
+lemma Linst.toXinst_toB8_eq_none {l : Linst} : l.toB8.toXinst = .none := by cases l <;> rfl
+lemma Linst.toJinst_toB8_eq_none {l : Linst} : l.toB8.toJinst = .none := by cases l <;> rfl
+lemma Linst.toLinst_toB8_eq_some {l : Linst} : l.toB8.toLinst = .some l := by cases l <;> rfl
 
-lemma Linst.toRinst_toB8_eq_none {l : Linst} : l.toB8.toRinst = .none := by
-  cases l <;> rfl
-
-lemma Linst.toXinst_toB8_eq_none {l : Linst} : l.toB8.toXinst = .none := by
-  cases l <;> rfl
-
-lemma Linst.toJinst_toB8_eq_none {l : Linst} : l.toB8.toJinst = .none := by
-  cases l <;> rfl
-
-lemma Linst.toLinst_toB8_eq_some {l : Linst} : l.toB8.toLinst = .some l := by
-  cases l <;> rfl
+lemma Jinst.toRinst_toB8_eq_none {j : Jinst} : j.toB8.toRinst = .none := by cases j <;> rfl
+lemma Jinst.toXinst_toB8_eq_none {j : Jinst} : j.toB8.toXinst = .none := by cases j <;> rfl
+lemma Jinst.toLinst_toB8_eq_none {j : Jinst} : j.toB8.toLinst = .none := by cases j <;> rfl
+lemma Jinst.toJinst_toB8_eq_some {j : Jinst} : j.toB8.toJinst = .some j := by cases j <;> rfl
 
 lemma none_mapRev {ξ υ} {f : ξ → υ} : (Option.none <&> f) = .none := by rfl
 
@@ -283,9 +553,8 @@ lemma Linst.getInst_of_slice {evm : Evm} {l : Linst} {xs : B8L}
   have rw := ByteArray.of_getElem?_eq_some eq
   have lt : evm.pc < evm.code.size := by
     simp only [ByteArray.size, Array.size]
-    rcases List.getElem?_eq_some_iff.mp eq with ⟨foo, bar⟩
-    rw [ByteArray.toList_eq_toList_data] at foo
-    apply foo
+    rcases List.getElem?_eq_some_iff.mp eq with ⟨lt, _⟩
+    rw [ByteArray.toList_eq_toList_data] at lt; exact lt
   rw [if_pos lt]
   conv => lhs; arg 1; lhs; rhs; rw [rw]; rfl
   rw [Linst.toRinst_toB8_eq_none, none_mapRev, none_orElse]
@@ -295,6 +564,52 @@ lemma Linst.getInst_of_slice {evm : Evm} {l : Linst} {xs : B8L}
   rw [Linst.toJinst_toB8_eq_none, none_mapRev, none_orElse]
   conv => lhs; arg 1; lhs; rhs; rw [rw]; rfl
   rw [Linst.toLinst_toB8_eq_some]; rfl
+
+lemma Jinst.at_of_slice {code : ByteArray} {pc} {j : Jinst}
+    (slice : code.toList.Slice pc [j.toB8]) : Jinst.At code pc j := by
+  have eq := List.get?_eq_of_slice slice
+  simp only [Jinst.At, ByteArray.getInst]
+  have rw := ByteArray.of_getElem?_eq_some eq
+  have lt : pc < code.size := by
+    simp only [ByteArray.size, Array.size]
+    rcases List.getElem?_eq_some_iff.mp eq with ⟨lt, _⟩
+    rw [ByteArray.toList_eq_toList_data] at lt; exact lt
+  rw [if_pos lt]
+  conv => lhs; arg 1; lhs; rhs; rw [rw]; rfl
+  rw [Jinst.toRinst_toB8_eq_none, none_mapRev, none_orElse]
+  conv => lhs; arg 1; lhs; rhs; rw [rw]; rfl
+  rw [Jinst.toXinst_toB8_eq_none, none_mapRev, none_orElse]
+  conv => lhs; arg 1; lhs; rhs; rw [rw]; rfl
+  rw [Jinst.toJinst_toB8_eq_some]; rfl
+
+lemma at_of_jumpable {code : ByteArray} {pc}
+    (jump : jumpable code pc = true) : Jinst.At code pc .jumpdest := by
+  unfold jumpable at jump
+  split at jump; rename_i h_get
+  · simp only [Jinst.At, ByteArray.getInst]
+    have lt : pc < code.size := by
+      by_contra h; simp only [not_lt] at h
+      have h_get0 : code.get! pc = 0 := by
+        simp only
+          [ByteArray.get!, Array.getElem!_eq_getD, Array.getD_eq_getD_getElem?]
+        rw [Array.getElem?_eq_none_iff.mpr h]; rfl
+      rw [h_get0] at h_get; cases h_get
+    rw [if_pos lt]
+    have r_none : B8.toRinst (code.get! pc) = none := by
+      rw [h_get]; apply Jinst.toRinst_toB8_eq_none
+    have x_none : B8.toXinst (code.get! pc) = none := by
+      rw [h_get]; apply Jinst.toXinst_toB8_eq_none
+    have j_some : B8.toJinst (code.get! pc) = some .jumpdest := by
+      rw [h_get]; apply Jinst.toJinst_toB8_eq_some
+    simp only [r_none, x_none, j_some, none_mapRev, none_orElse]
+    rfl
+  · cases jump
+
+def PushAt (code : ByteArray) (pc : Nat) (xs : B8L) : Prop :=
+  ∃ le : xs.length ≤ 32, code.getInst pc = some (.next (.push xs le))
+
+lemma pushAt_of_slice {code : ByteArray} {pc} {xs : B8L}
+    (slice : code.toList.Slice pc (pushToB8L xs)) : PushAt code pc xs := sorry
 
 lemma Ninst.getInst_of_slice {evm : Evm} {n : Ninst} :
     evm.code.toList.Slice evm.pc n.toB8L → n.At evm.code evm.pc := by sorry
@@ -313,7 +628,7 @@ lemma Ninst.inv_code {n} : Ninst.Inv Evm.code n := by sorry
 lemma Ninst.run_of_at {evm n exn}
     (ex : Exec evm exn) (h_at : n.At evm.code evm.pc) :
     ∃ (evm' : Evm) (ex' : Exec evm' exn)
-      (rel : Exec'.Rel ⟨evm', exn, ex'⟩ ⟨evm, exn, ex⟩),
+      (rel : Pack.Rel ⟨evm', exn, ex'⟩ ⟨evm, exn, ex⟩),
       evm'.pc = evm.pc + n.toB8L.length ∧ Ninst.Run evm n evm' := sorry
 
 -- lemma Ninst.run_of_at {e s pc i r}
@@ -362,14 +677,12 @@ lemma Evm.getInst_eq_getInst' {evm : Evm} : evm.getInst = evm.getInst' evm.pc :=
 -- def Jinst.At' (evm : Evm) (pc : Nat) (j : Jinst) : Prop :=
   -- evm.getInst' pc = some (.jump j)
 
-def PushAt (evm : Evm) (pc : Nat) (xs : B8L) : Prop :=
-  ∃ le : xs.length ≤ 32, evm.getInst' pc = some (.next (.push xs le))
 
 lemma subcode_compile_branch {evm : Evm} {k l p q}
     (h : subcode evm.code.toList k (Func.compile l k (Func.branch p q))) :
     ∃ loc : Nat,
       loc < 2 ^ 16 ∧
-      PushAt evm k [(loc >>> 8).toUInt8, loc.toUInt8] ∧
+      PushAt evm.code k [(loc >>> 8).toUInt8, loc.toUInt8] ∧
       Jinst.jumpi.At evm.code (k + 3) ∧
       subcode evm.code.toList (k + 4) (Func.compile l (k + 4) p) ∧
       Jinst.jumpdest.At evm.code loc ∧
@@ -380,11 +693,12 @@ lemma jumpi_at {evm exn} (ex : Exec evm exn) (h : Jinst.jumpi.At evm.code evm.pc
     ( ∃ (x : B256) (evm' : Evm) (ex' : Exec evm' exn),
         evm'.pc = evm.pc + 1 ∧
         Evm.Pop [x, 0] evm evm' ∧
-        Exec'.Rel ⟨evm', exn, ex'⟩ ⟨evm, exn, ex⟩ ) ∨
+        Pack.Rel ⟨evm', exn, ex'⟩ ⟨evm, exn, ex⟩ ) ∨
     ( ∃ (x y : B256) (evm' : Evm) (ex' : Exec evm' exn),
+        evm'.pc = x.toNat ∧
         Evm.Pop [x, y] evm evm' ∧
-        --Jumpable e x.toNat ∧ y ≠ 0 ∧
-        Exec'.Rel ⟨evm', exn, ex'⟩ ⟨evm, exn, ex⟩ ) := by
+        jumpable evm.code x.toNat ∧ y ≠ 0 ∧
+        Pack.Rel ⟨evm', exn, ex'⟩ ⟨evm, exn, ex⟩ ) := by
   -- rcases Jinst.run_of_at cr h with ⟨s', pc', cr', h_run, h_prec⟩
   -- cases h_run
   -- · left; refine ⟨_, _, asm, asm, h_prec⟩
@@ -421,19 +735,690 @@ lemma Evm.push_cons_pop_cons
     {g with stack := h_pop}
   ⟩
 
-infix:70 " ≅ "  => Evm.Rel Evm.Rels.eqs
+def Evm.Equiv (evm evm' : Evm) : Prop :=
+  Evm.Rel Evm.Rels.equiv evm evm'
+
+infix:70 " ≅ "  => Evm.Equiv
 
 lemma Evm.push_nil {evm evm'} (h : Evm.Push [] evm evm') : evm ≅ evm' := by
   have h_stk : evm.stack = evm'.stack := h.stack.symm
   exact {h with stack := h_stk}
 
+lemma rel_of_rel_of_equiv {evm evm' evm''} {rs : Evm.Rels}
+    (rel : Evm.Rel rs evm evm') (equiv : evm' ≅ evm'') :
+    Evm.Rel rs evm evm'' := by
+  constructor
+  · rw [← equiv.stack]; exact rel.stack
+  · rw [← equiv.memory]; exact rel.memory
+  · rw [← equiv.code]; exact rel.code
+  · rw [← equiv.logs]; exact rel.logs
+  · rw [← equiv.msg]; exact rel.msg
+  · rw [← equiv.output]; exact rel.output
+  · rw [← equiv.returnData]; exact rel.returnData
+  · rw [← equiv.error]; exact rel.error
+
+lemma rel_of_equiv_of_rel {evm evm' evm''} {rs : Evm.Rels}
+    (equiv : evm ≅ evm') (rel : Evm.Rel rs evm' evm'') :
+    Evm.Rel rs evm evm'' := by
+  constructor
+  · rw [equiv.stack]; exact rel.stack
+  · rw [equiv.memory]; exact rel.memory
+  · rw [equiv.code]; exact rel.code
+  · rw [equiv.logs]; exact rel.logs
+  · rw [equiv.msg]; exact rel.msg
+  · rw [equiv.output]; exact rel.output
+  · rw [equiv.returnData]; exact rel.returnData
+  · rw [equiv.error]; exact rel.error
+
+
+lemma push_of_pushAt {evm bs exn} (cr : Exec evm exn)
+    (h_at : PushAt evm.code evm.pc bs) :
+    ∃ (evm' : Evm) (cr' : Exec evm' exn),
+      evm'.pc = evm.pc + bs.length + 1 ∧
+      Evm.Push [B8L.toB256 bs] evm evm' ∧
+      Pack.Rel ⟨evm', exn, cr'⟩ ⟨evm, exn, cr⟩ := by
+  sorry
+
+-- lemma push_of_pushAt {e s pc bs r} (cr : Exec e s pc r) (h_at :PushAt e pc bs) :
+--     ∃ (s' : Desc) (cr' : Exec e s' (pc + bs.length + 1) r),
+--       Desc.Push [B8L.toB256 bs] s s' ∧
+--       Exec'.Rel ⟨e, s', pc + bs.length + 1, r, cr'⟩ ⟨e, s, pc, r, cr⟩ := by
+--   cases cr with
+--   | step =>
+--     rename Desc => s'; refine' ⟨s', _⟩
+--     have h_prec := Exec'.Rel.step asm asm
+--     rename Step _ _ _ _ _ => h_step; cases h_step
+--     · cases not_pushAt_of_op_at  asm h_at
+--     · cases not_pushAt_of_cop_at asm h_at
+--     · cases not_pushAt_of_cop_at asm h_at
+--     · cases not_pushAt_of_jop_at asm h_at
+--     · rename (PushAt e pc _) => h_at'
+--       cases pushAt_unique h_at h_at'
+--       refine' ⟨_, asm, h_prec⟩
+--   | exec =>
+--     cases not_pushAt_of_cop_at asm h_at
+--   | halt =>
+--     rename Halt _ _ _ _ => h_halt; cases h_halt
+--     · cases not_pushAt_of_hop_at asm h_at
+--     · cases List.not_slice_length h_at.left
+
+lemma Nat.lo_eq (m n : Nat) : m ↾ n = m % (2 ^ n) := rfl
+lemma Nat.hi_eq (m n : Nat) : m ↿ n = (m >>> n) <<< n := rfl
+
+lemma B32.ofNat_eq_iff_mod_eq_toNat (a : Nat) (b : B32) :
+    a.toB32 = b ↔ a ↾ 32 = b.toNat :=
+  UInt32.ofNat_eq_iff_mod_eq_toNat a b
+
+lemma Nat.toB16_toB8 (n : Nat) : n.toB8.toB16 = (n ↾ 8).toB16 := by sorry
+
+lemma Nat.toB32_toB16 (n : Nat) : n.toB16.toB32 = (n ↾ 16).toB32 := by
+  have h0 : n.toB16.toB32 = n.toB32 % (2 ^ 16) :=
+      (UInt16.toUInt32_eq_mod_65536_iff n.toUInt16 n.toUInt32).mpr
+        (UInt32.toUInt16_ofNat' _).symm
+  have h1: (n.toB32 % 2 ^ 16).toNat = n ↾ 16 := by
+    have rw : B32.toNat (2 ^ 16) = 2 ^ 16 := rfl
+    rw [B32.toNat_mod, rw]; clear rw
+    rw [toNat_toB32, ← Nat.lo_eq]
+    apply Nat.lo_lo_of_ge (by omega)
+  have h2 : (n ↾ 16).toB32 = n.toB32 % (2 ^ 16) := by
+    apply (B32.ofNat_eq_iff_mod_eq_toNat _ _).mpr
+    apply Eq.trans (Nat.lo_lo_of_le (by omega)) h1.symm
+  apply Eq.trans h0 h2.symm
+
+lemma Nat.toB64_toB32 (n : Nat) : n.toB32.toB64 = (n ↾ 32).toB64 := by
+  have h0 : n.toB32.toB64 = n.toB64 % (2 ^ 32) :=
+      (UInt32.toUInt64_eq_mod_4294967296_iff n.toUInt32 n.toUInt64).mpr
+        (UInt64.toUInt32_ofNat' _).symm
+  have h1: (n.toB64 % 2 ^ 32).toNat = n ↾ 32 := by
+    have rw : B64.toNat (2 ^ 32) = 2 ^ 32 := rfl
+    rw [B64.toNat_mod, rw]; clear rw
+    rw [toNat_toB64, ← Nat.lo_eq]
+    apply Nat.lo_lo_of_ge (by omega)
+  have h2 : (n ↾ 32).toB64 = n.toB64 % (2 ^ 32) := by
+    apply (B64.ofNat_eq_iff_mod_eq_toNat _ _).mpr
+    apply Eq.trans (Nat.lo_lo_of_le (by omega)) h1.symm
+  apply Eq.trans h0 h2.symm
+lemma toNat_toB16 {n : Nat} : n.toB16.toNat = n ↾ 16 := UInt16.toNat_ofNat'
+
+lemma pair_aux (n m : Nat) :
+    ((n >>> m ↾ m) ↾ (m + m)) <<< m ↾ (m + m) ||| (n ↾ m) ↾ (m + m) =
+      n ↾ (m + m) := by
+  rw [Nat.lo_lo_of_le (by omega)]
+  rw [Nat.lo_lo_of_le (by omega)]
+  apply Eq.trans _ <| high_or_low_eq_self (n ↾ (m + m)) m Nat.lo_lt
+  apply congr_arg₂  _ _ (Nat.lo_lo_of_ge (by omega)).symm
+  rw [@Nat.lo_add_shr n m m, ← Nat.lo_eq _ m, Nat.lo_lo]; rfl
+
+lemma List.toB16_pair (n : Nat) :
+    B8L.toB16 [(n >>> 8).toB8, n.toB8] = n.toB16 := by
+  have h : (n >>> 8 ↾ 8).toB16 <<< 8 ||| (n ↾ 8).toB16 = n.toB16 := by
+    rw [← B16.toNat_inj, toNat_toB16, B16.toNat_or, toNat_toB16]
+    rw [B16.toNat_shiftLeft, toNat_toB16]; apply pair_aux n 8
+  simp [B8L.toB16, B8L.pack, ekatD, takeD, reverse, reverseAux, tail, headD]
+  rw [Nat.toB16_toB8, Nat.toB16_toB8, h]
+
+lemma B32.toNat_shl (a b : B32) :
+    (a <<< b).toNat = a.toNat <<< (b.toNat % 32) ↾ 32 :=
+  UInt32.toNat_shiftLeft a b
+
+lemma B64.toNat_shl (a b : B64) :
+    (a <<< b).toNat = (a.toNat <<< (b.toNat % 64)) ↾ 64 :=
+  UInt64.toNat_shiftLeft a b
+
+def B16.concat (x y : B16) : B32 :=
+  x.toB32 <<< 16 ||| y.toB32
+
+def B32.concat (x y : B32) : B64 :=
+  x.toB64 <<< 32 ||| y.toB64
+
+lemma Nat.hi_le (a b : Nat) : a ↿ b ≤ a := by
+  rw [hi, shiftLeft_eq, shiftRight_eq_div_pow]
+  apply Nat.div_mul_le_self
+
+lemma toB32_eq_concat (n : Nat) :
+    n.toB32 = B16.concat (n >>> 16).toB16 n.toB16 := by
+  rw [← B32.toNat_inj, toNat_toB32]
+  simp only [B16.concat, Nat.toB32_toB16]
+  rw [B32.toNat_or, B32.toNat_shl, toNat_toB32, toNat_toB32]
+  rw [Nat.lo_lo_of_le (by omega), Nat.lo_lo_of_le (by omega)]
+  have rw : (B32.toNat 16 % 32) = 16 := rfl
+  rw [rw]; clear rw
+  have rw : (n >>> 16 ↾ 16) <<< 16 ↾ 32 = (n ↾ 32) ↿ 16 := by
+    rw [← Nat.lo_add_shr, ← Nat.hi_eq]
+    apply Nat.lo_eq_of_lt
+    apply lt_of_le_of_lt (Nat.hi_le _ _) Nat.lo_lt
+  rw [rw, ← @Nat.lo_lo_of_ge n 32 16 (by omega)]
+  apply (Nat.hi_or_lo _ _).symm
+
+lemma toB64_eq_concat (n : Nat) :
+    n.toB64 = B32.concat (n >>> 32).toB32 n.toB32 := by
+  rw [← B64.toNat_inj, toNat_toB64]
+  simp only [B32.concat, Nat.toB64_toB32]
+  rw [B64.toNat_or, B64.toNat_shl, toNat_toB64, toNat_toB64]
+  rw [Nat.lo_lo_of_le (by omega), Nat.lo_lo_of_le (by omega)]
+  have rw : (B64.toNat 32 % 64) = 32 := rfl
+  rw [rw]; clear rw
+  have rw : (n >>> 32 ↾ 32) <<< 32 ↾ 64 = (n ↾ 64) ↿ 32 := by
+    rw [← Nat.lo_add_shr, ← Nat.hi_eq]
+    apply Nat.lo_eq_of_lt
+    apply lt_of_le_of_lt (Nat.hi_le _ _) Nat.lo_lt
+  rw [rw, ← @Nat.lo_lo_of_ge n 64 32 (by omega)]
+  apply (Nat.hi_or_lo _ _).symm
+
+lemma List.toB32_pair (n : Nat) (n_lt : n < 2 ^ 16) :
+    B8L.toB32 [(n >>> 8).toB8, n.toB8] = n.toB32 := by
+  simp only [ B8L.toB32, B8L.pack, ekatD, takeD,
+    reverse, reverseAux, tail, headD, take, drop ]
+  apply Eq.trans _ (toB32_eq_concat _).symm
+  apply congr_arg₂ _ _ (congr_arg _ _)
+  · apply congr_arg (λ x : B32 => x <<< 16) <| congr_arg _ _
+    rw [Nat.shiftRight_eq_div_pow, Nat.div_eq_zero_of_lt (by omega)]; rfl
+  · apply List.toB16_pair
+
+lemma List.toB64_pair (n : Nat) (n_lt : n < 2 ^ 16) :
+    B8L.toB64 [(n >>> 8).toB8, n.toB8] = n.toB64 := by
+  simp only [ B8L.toB64, B8L.pack, ekatD, takeD,
+    reverse, reverseAux, tail, headD, take, drop ]
+  apply Eq.trans _ (toB64_eq_concat _).symm
+  apply congr_arg₂ _ _ (congr_arg _ _)
+  · apply congr_arg (λ x : B64 => x <<< 32) <| congr_arg _ _
+    rw [Nat.shiftRight_eq_div_pow, Nat.div_eq_zero_of_lt (by omega)]; rfl
+  · apply List.toB32_pair _ n_lt
+
+lemma List.toB128_pair (n : Nat) (n_lt : n < 2 ^ 16):
+    B8L.toB128 [(n >>> 8).toUInt8, n.toUInt8] = n.toB128 := by
+  apply @Eq.trans _ _ ⟨0, n.toB64⟩
+  · apply @Eq.trans _ _ ⟨0, B8L.toB64 [(n >>> 8).toUInt8, n.toUInt8]⟩
+    · simp [B8L.toB128, List.ekatD, B8L.pack]
+      apply congr_arg₂ _ rfl rfl
+    · apply congr_arg₂ _ rfl <| List.toB64_pair _ n_lt
+  · simp only [Nat.toB128]; apply congr_arg₂ _ _ rfl
+    rw [Nat.shiftRight_eq_zero _ _ (by omega)]; rfl
+lemma List.toB256_pair (n : Nat) (n_lt : n < 2 ^ 16):
+    B8L.toB256 [(n >>> 8).toUInt8, n.toUInt8] = n.toB256 := by
+  apply @Eq.trans _ _ ⟨0, n.toB128⟩
+  · apply @Eq.trans _ _ ⟨0, B8L.toB128 [(n >>> 8).toUInt8, n.toUInt8]⟩
+    · simp [B8L.toB256, List.ekatD, B8L.pack]
+      apply congr_arg₂ _ rfl rfl
+    · apply congr_arg₂ _ rfl <| List.toB128_pair _ n_lt
+  · simp only [Nat.toB256]; apply congr_arg₂ _ _ rfl
+    rw [Nat.shiftRight_eq_zero _ _ (by omega)]; rfl
+
+lemma toNat_toB256 (n : Nat) : n.toB256.toNat = n ↾ 256 := by
+  simp only [Nat.toB256, B256.toNat]; rw [toNat_toB128, toNat_toB128]
+  apply Nat.or_eq_lo_add
+
+lemma toNat_toB256_of_lt {n : Nat} (h : n < 2 ^ 256) : n.toB256.toNat = n := by
+  rw [toNat_toB256, Nat.lo_eq_of_lt h]
+
+lemma Jinst.run_of_at {evm exn o}
+    (cr : Exec evm exn) (h_at : Jinst.At evm.code evm.pc o) :
+    ∃ (evm' : Evm) (cr' : Exec evm' exn),
+      Jinst.Run' evm o (.ok evm') ∧
+      Pack.Rel ⟨evm', exn, cr'⟩ ⟨evm, exn, cr⟩ := by
+  sorry
+
+class HPrsv (f : Evm → Execution) where
+  (prsv : ∀ {evm evm'}, f evm = .ok evm' → evm ≅ evm')
+
+instance {gas} : HPrsv (chargeGas gas) := by
+  constructor; intros evm evm' h
+  simp only [chargeGas] at h; split at h; {cases h}
+  injection h with rw; rw [← rw]
+  constructor <;> rfl
+
+instance : HPrsv Evm.incrPc := by
+  constructor; intros evm evm' h
+  simp only [Evm.incrPc] at h
+  injection h with rw; rw [← rw]
+  constructor <;> rfl
+
+lemma chargeGas_inv_pc {gas : Nat} {evm evm' : Evm} :
+    chargeGas gas evm = .ok evm' → evm.pc = evm'.pc := by
+  simp only [chargeGas]; split <;> intro h
+  · cases h
+  · rw [← Except.ok.inj h]
+
+lemma exec_inv_code {evm evm' : Evm} :
+    Exec evm (.ok evm') → evm.code = evm'.code := by
+  sorry
+
+
+lemma Evm.equiv_trans {evm evm' evm''}
+    (h₁ : Evm.Equiv evm evm') (h₂ : Evm.Equiv evm' evm'') :
+    Evm.Equiv evm evm'' := by
+  constructor
+  · rw [h₁.stack, h₂.stack]; rfl
+  · rw [h₁.memory, h₂.memory]; rfl
+  · rw [h₁.code, h₂.code]; rfl
+  · rw [h₁.logs, h₂.logs]; rfl
+  · rw [h₁.msg, h₂.msg]; rfl
+  · rw [h₁.output, h₂.output]; rfl
+  · rw [h₁.returnData, h₂.returnData]; rfl
+  · rw [h₁.error, h₂.error]; rfl
+
+lemma incrPc_incr_pc {evm evm' : Evm} :
+    evm.incrPc = .ok evm' → evm.pc + 1 = evm'.pc := by
+  simp only [Evm.incrPc]; intro h; rw [← Except.ok.inj h]
+
+lemma Evm.pop_of_pop {evm evm' : Evm} {x}
+    (pop : Evm.pop evm = .ok ⟨x, evm'⟩) : Evm.Pop [x] evm evm' := by
+  simp only [Evm.pop] at pop; split at pop; {cases pop}
+  injection pop with eq; injection eq with eq eq'
+  constructor <;> simp <;> rw [← eq'] <;> try {rfl}
+  rename (evm.stack = _) => rw; rw [rw, eq]; rfl
+
+lemma jumpdest_at {evm exn} (cr : Exec evm exn)
+    (h : Jinst.At evm.code evm.pc Jinst.jumpdest) :
+    ∃ (evm' : Evm) (cr' : Exec evm' exn),
+      evm ≅ evm' ∧
+      evm'.pc = evm.pc + 1 ∧
+      Pack.Rel ⟨evm', exn, cr'⟩ ⟨evm, exn, cr⟩ := by
+  rcases Jinst.run_of_at cr h with ⟨evm', exn', h_run, h_prec⟩
+  simp only [Jinst.Run', Jinst.run] at h_run
+
+  have eqv : evm ≅ evm' := by
+    rcases of_bind_eq_ok h_run with ⟨evm_mid, eq, eq'⟩
+    apply @Evm.equiv_trans _ evm_mid
+    · apply HPrsv.prsv eq
+    · apply HPrsv.prsv eq'
+  refine' ⟨evm', exn', eqv, _, h_prec⟩
+  rcases of_bind_eq_ok h_run with ⟨evm_gas, eq, eq'⟩
+  rw [chargeGas_inv_pc eq, incrPc_incr_pc eq']
+
+lemma Except.of_assert_eq_ok {p : Prop} [Decidable p] {ξ} {x : ξ}
+    (h : Except.assert p x = .ok ()) : p := by
+  simp [Except.assert] at h; apply h
+
+lemma jump_at {s r} (cr : Exec s r)
+    (h : Jinst.At s.code s.pc Jinst.jump) :
+    ∃ (x : B256) (s' : Evm) (cr' : Exec s' r),
+      s'.pc = x.toNat ∧
+      Evm.Pop [x] s s' ∧
+      jumpable s.code x.toNat = true ∧
+      Pack.Rel ⟨s', r, cr'⟩ ⟨s, r, cr⟩ := by
+  rcases Jinst.run_of_at cr h with ⟨s_j, cr_j, h_run, h_prec⟩
+  simp only [Jinst.Run', Jinst.run] at h_run
+  rcases of_bind_eq_ok h_run with ⟨⟨loc, s'⟩, pop_eq, run'⟩; clear h_run
+  rcases of_bind_eq_ok run' with ⟨s'', cg_eq, run''⟩; clear run'
+  rcases of_bind_eq_ok run'' with ⟨u, asrt_eq, run'''⟩; clear run''
+  have pop := Evm.pop_of_pop pop_eq
+  have eqv := (HPrsv.prsv cg_eq)
+  injection run''' with rw
+  refine' ⟨loc, s_j, cr_j, _, _, _, h_prec⟩
+  · rw [← rw]
+  · have eqv' : s'' ≅ s_j := by
+      rw [← rw]; constructor <;> rfl
+    apply rel_of_rel_of_equiv _ eqv'
+    apply rel_of_rel_of_equiv pop eqv
+  · have hh := Except.of_assert_eq_ok asrt_eq
+    rw [pop.code, eqv.code]; apply Except.of_assert_eq_ok asrt_eq
+
+lemma of_guard_eq_some {p : Prop} [hd : Decidable p] {ξ} {ox : Option ξ} {x} :
+    (do guard p; ox) = some x → p ∧ ox = some x := by
+  intro h
+  cases em p with
+  | inl hp => simp [hp] at h; constructor <;> assumption
+  | inr hp => simp [guard, if_neg hp] at h
+
+lemma subcode_compile_call {code : ByteArray} {l m n}
+  (h : subcode code.toList m (Func.compile l m (Func.call n))) :
+    ∃ (loc : Nat) (p : Func),
+      l[n]? = some (loc, p) ∧
+      loc < 2 ^ 16 ∧
+      PushAt code m ([(loc >>> 8).toUInt8, loc.toUInt8]) ∧
+      Jinst.jump.At code (m + 3) := by
+  rcases of_subcode h with ⟨cd, h', h_slice⟩; clear h
+  rcases of_bind_eq_some h' with ⟨⟨loc, p⟩, h_get, h⟩; clear h'
+  simp at h
+  rcases of_guard_eq_some h with ⟨h_lt, h_eq⟩; clear h
+  refine' ⟨loc, p, h_get, h_lt, _⟩
+  simp at h_eq; rw [← h_eq] at h_slice
+  refine' ⟨
+    @pushAt_of_slice code m
+      [UInt8.ofNat (loc >>> 8), UInt8.ofNat loc]
+      (List.slice_prefix h_slice),
+    _
+  ⟩
+  have slice : code.toList.Slice (m + 3) [Jinst.jump.toB8] :=
+    @List.slice_suffix _ code.toList m [_ ,_, _] _ h_slice
+  apply @Jinst.at_of_slice code (m + 3) .jump slice
+
+lemma Prog.get?_table {m n} {c : List Func} :
+    (Prod.snd <$> (table m c)[n]? : Option Func) =
+      ((@getElem? (List Func) Nat Func _ _ c n) : Option Func) := by
+  induction c generalizing m n with
+  | nil => rfl
+  | cons p c' ih =>
+    cases n with
+    | zero => simp [table]
+    | succ n => simp [table]; apply ih
+
+lemma List.of_get?_succ_eq_some {X} {l : List X} {k x} :
+    l[k + 1]? = some x → ∃ y, l[k]? = some y := by
+  induction k generalizing l x with
+  | zero =>
+    match l with
+    | [] => simp
+    | [_] => simp
+    | (y :: _ :: _) => intro _; refine' ⟨y, rfl⟩
+  | succ k ih =>
+    match l with
+    | [] => simp
+    | (_ :: l') =>
+      intro h_get; apply ih h_get
+
+lemma table_suffix {c k pfx sfx} (h : pfx <++ (table k c) ++> sfx) :
+    ∃ k' c', sfx = table k' c' := by
+  induction c generalizing k pfx sfx with
+  | nil => refine' ⟨k, [], (List.append_eq_nil_iff.mp h.symm).right⟩
+  | cons p ps ih =>
+    simp [table] at h
+    rcases List.cons_eq_append_iff.mp h with
+      ⟨_, h'⟩ | ⟨pfx', _, h'⟩
+    · refine ⟨k, p :: ps, h'⟩
+    · exact ih h'
+
+lemma Func.length_compile {l k p bs} (h : Func.compile l k p = some bs) :
+    bs.length = compsize p := by
+  induction p generalizing k bs with
+  | branch p q ihp ihq =>
+    rcases of_bind_eq_some h with ⟨cp, h_cp, h'⟩; clear h
+    rcases of_guard_eq_some h' with ⟨h'', h⟩; clear h' h''
+    rcases of_bind_eq_some h with ⟨cq, h_cq, h'⟩; clear h
+    simp at h'; rw [← h']
+    simp [List.length_append, List.length, compsize]
+    rw [ihp h_cp, ihq h_cq]; omega
+  | last o => simp [compile] at h; rw [← h]; rfl
+  | next o p ih =>
+    rcases of_bind_eq_some h with ⟨bs', h, h'⟩;
+    simp at h'; rw [← h']
+    simp [List.length_append, compsize]
+    rw [ih h, Nat.add_comm]
+  | call m =>
+    rcases of_bind_eq_some h with ⟨⟨_, _⟩, _, h'⟩; clear h
+    rcases of_guard_eq_some h' with ⟨h'', h⟩; clear h' h''
+    simp at h; rw [← h];
+    simp [List.length, compsize]
+
+lemma of_get?_table_eq_some {f fs} {bs} {m n : ℕ} {p : Func}
+    (h_eq : some bs = Prog.compile ⟨f, fs⟩)
+    (h_get : (table 0 (f :: fs))[m]? = some (n, p)) :
+    ∃ lft rgt,
+      lft.length = m ∧
+      (lft <++ (table 0 (f :: fs)) ++> ((n, p) :: rgt)) ∧
+    ∃ pfx sfx,
+      pfx.length = n ∧
+      (pfx <++ bs ++> sfx) ∧
+      (some sfx = Table.compile (table 0 (f :: fs)) ((n, p) :: rgt)) := by
+  revert n p h_get
+  induction m with
+  | zero =>
+    intro n p h_get
+    simp [table] at h_get
+    cases h_get.left; cases h_get.right; clear h_get
+    simp only [table]
+    refine' ⟨ [], _ , rfl, List.nil_append _, [],
+              bs, rfl, (List.nil_append _).symm, _ ⟩
+    rw [h_eq]; simp [Prog.compile, table]
+  | succ m ih =>
+    intro n p h_get
+    rcases List.of_get?_succ_eq_some h_get with ⟨⟨k, q⟩, h⟩
+    rcases ih h with
+      ⟨lft, rgt, h_lft, h_split, pfx, sfx, h_pfx, h_split', h_sfx⟩
+    clear ih h
+    refine' ⟨lft ++ [(k, q)], _⟩
+    have h : ∃ rgt', rgt = (n, p) :: rgt' := by
+      have h_sub : m.succ - m = 1 := by omega
+      have h_le : List.length lft ≤ Nat.succ m := by
+        rw [h_lft]; apply Nat.le_succ
+      have heq : (lft ++ (k, q) :: rgt)[m.succ]? = ((k, q) :: rgt)[m.succ - lft.length]? := by
+        simp [List.getElem?_append_right, h_le]
+      rw [h_split, heq, h_lft, h_sub] at h_get
+      match rgt with
+      | [] => simp  at h_get
+      | _ :: rgt' =>
+        simp at h_get
+        rw [h_get]; refine ⟨_, rfl⟩
+    rcases h with ⟨rgt', h_rgt'⟩
+    refine' ⟨rgt', _, _, _⟩
+    · simp [List.length, h_lft]
+    · simp [Split]; rw [← h_rgt', h_split]
+    · rcases Table.compile_cons_eq_some h_sfx.symm with
+        ⟨cq, cl, h_cq, h_cl, h_sfx'⟩
+      refine' ⟨pfx ++ ([Jinst.jumpdest.toB8] ++ cq), cl, _, _, _⟩
+      · have hn : n = k + compsize q + 1 := by
+          rcases table_suffix h_split with
+            ⟨k', _ | ⟨q', c'⟩, h⟩ <;> simp [table] at h
+          rcases h with ⟨⟨⟨_⟩,⟨_⟩⟩, h⟩
+          rw [h_rgt'] at h
+          cases c' <;> simp [table] at h
+          apply h.left.left
+        simp [List.length_append, List.length]
+        rw [h_pfx, hn, Func.length_compile h_cq]
+        omega
+      · simp only [Split]; rw [List.append_assoc, ← h_sfx', h_split']
+      · rw [← h_cl, ← h_rgt']
+
+lemma subcode_of_get?_eq_some {f fs} {code : ByteArray} {k loc : ℕ} {p : Func}
+    (h_eq : some code.toList = Prog.compile ⟨f, fs⟩)
+    (h_get : getElem? (table 0 (f :: fs)) k = some ⟨loc, p⟩) :
+    Jinst.At code loc Jinst.jumpdest ∧
+    subcode code.toList (loc + 1) (Func.compile (table 0 (f :: fs)) (loc + 1) p) := by
+  rcases of_get?_table_eq_some h_eq h_get with
+    ⟨lft, rgt, _, _, pfx, sfx, h_pfx, h_split', h_sfx⟩
+  unfold Jinst.At
+  rcases Table.compile_cons_eq_some h_sfx.symm with ⟨bs, bs', h_bs, _, h_sfx'⟩
+  have h_slice : List.Slice code.toList loc sfx := by
+    rw [← h_pfx, h_split']; apply List.append_slice_suffix
+  rw [h_sfx', List.append_assoc] at h_slice
+  constructor
+  · apply Jinst.at_of_slice
+    apply List.slice_prefix h_slice
+  · rw [h_bs]; simp [subcode]
+    apply List.slice_prefix <| List.slice_suffix h_slice
+
 theorem correct_core (f : Func) (fs : List Func) :
-    ∀ (pk : Exec') (p : Func),
+    ∀ (pk : Pack) (p : Func) (tevm : Evm),
+      some pk.evm.code.toList = Prog.compile ⟨f, fs⟩ →
+      subcode pk.evm.code.toList pk.evm.pc
+        (Func.compile (table 0 (f :: fs)) pk.evm.pc p) →
+      pk.exn = .ok tevm →
+      Func.Run (f :: fs) pk.evm p tevm := by
+  apply Pack.strongRec; intro pk ih p tevm eq sc eq_tevm
+  match p with
+  | .last o =>
+    apply Func.Run.last; rw [← eq_tevm]
+    apply Linst.run_of_at pk.ex <| Linst.getInst_of_slice sc
+  | .next n p =>
+    rcases of_subcode sc with ⟨cd, h_eq', h_slice⟩; clear sc
+    rcases of_bind_eq_some h_eq' with ⟨cd', h_eq'', h_rw⟩; clear h_eq'
+    simp [pure] at h_rw; rw [← h_rw] at h_slice; clear h_rw cd
+    have h_at : n.At pk.evm.code pk.evm.pc := by
+      apply Ninst.getInst_of_slice; apply List.slice_prefix h_slice
+    rcases Ninst.run_of_at pk.ex h_at with ⟨evm', ex', h_prec, h_pc, h_run⟩
+    have h_run' : Func.Run (f :: fs) evm' p tevm := by
+      apply ih ⟨evm', pk.exn, ex'⟩ (Pack.lt_of_prec h_prec) p
+      · simp; rw [← Ninst.inv_code h_run]; apply eq
+      · simp; rw [h_pc, h_eq'', ← Ninst.inv_code h_run]
+        apply List.slice_suffix h_slice
+      · apply eq_tevm
+    apply Func.Run.next h_run h_run'
+  | .branch p q => sorry
+  | .call k =>
+    rcases subcode_compile_call sc with ⟨loc, p, h_get, h_loc, h_push, h_jump⟩
+    have h_get' : (f :: fs)[k]? = p := by
+      rw [← @Prog.get?_table 0 k (f :: fs), h_get]; rfl
+
+    apply Func.Run.call h_get'
+
+
+
+    have h :
+        ∃ (s' : Evm) (cr' : Exec s' pk.exn),
+          s'.pc = pk.evm.pc + 3  ∧
+          Evm.Push [loc.toB256] pk.evm s' ∧
+          Pack.Rel ⟨s', pk.exn, cr'⟩ pk := by
+      sorry
+
+
+    clear h_push; rcases h with ⟨s, cr, h_pc, h_push, h_prec⟩
+
+    have h_jump' : Jinst.At s.code s.pc Jinst.jump := by
+      rw [← h_push.code, h_pc]; apply h_jump
+    rcases jump_at cr h_jump' with ⟨x, s', cr', h_pc', h_pop, h, h_prec'⟩
+    have h_jumpable : Jinst.At s'.code s'.pc Jinst.jumpdest := by
+      rw [← h_pop.code, h_pc']; apply at_of_jumpable h;
+
+    clear h;
+
+    rcases subcode_of_get?_eq_some eq h_get with ⟨h, hp⟩; clear h
+
+    rcases jumpdest_at cr' h_jumpable with ⟨s'', cr'', eqv'', h_pc'', h_prec''⟩
+
+
+    have h_lt : Pack.lt ⟨s'', pk.exn, cr''⟩ pk := by sorry
+
+    have hh := ih ⟨s'', pk.exn, cr''⟩ h_lt p tevm sorry sorry --hp
+
+
+
+
+
+
+
+
+
+
+
+
+
+
+
+
+
+
+   --  rcases subcode_compile_call h_sub with ⟨loc, p, h_get, h_loc, h_push, h_jump⟩
+   --  have h_get' : (f :: fs)[k]? = p := by
+   --    rw [← @Prog.get?_table 0 k (f :: fs), h_get]; rfl
+   --  apply Func.Run.call h_get'
+   --  have h :
+   --    ∃ (s' : Desc) (cr' : Exec pk.e s' (pk.pc + 3) pk.r),
+   --      Desc.Push [loc.toB256] pk.s s' ∧
+   --      Exec'.Rel ⟨pk.e, s', pk.pc + 3, pk.r, cr'⟩ pk := by
+   --    rcases push_of_pushAt pk.cr h_push with ⟨s', cr', h, h_prec⟩
+   --    rw [List.toB256_pair _ h_loc] at h
+   --    refine' ⟨s', cr', h, h_prec⟩
+   --  clear h_push; rcases h with ⟨s, cr, h_push, h_prec⟩
+   --  rcases jump_at cr h_jump with ⟨x, s', cr', h_pop, h, h_prec'⟩
+   --  rcases h with ⟨h_jumpable, h⟩; clear h
+   --  rcases subcode_of_get?_eq_some h_eq h_get with ⟨h, hp⟩; clear h
+   --  rcases jumpdest_at cr' h_jumpable with ⟨cr'', h_prec''⟩
+   --  have h_loc' : loc < 2 ^ 256 := by
+   --    apply Nat.lt_trans h_loc
+   --    rw [Nat.pow_lt_pow_iff_right] <;> omega
+   --  have h : loc = x.toNat ∧ pk.s = s' := by
+   --    rcases Desc.push_cons_pop_cons h_push h_pop with ⟨hx, st, h_push', h_pop'⟩
+   --    rw [Desc.push_nil h_push', Desc.pop_nil h_pop']
+   --    rw [← congrArg B256.toNat hx, toNat_toB256_of_lt h_loc']; simp
+   --  rcases h with ⟨h_rw, h_rw'⟩
+   --  rw [h_rw']; rw [h_rw] at hp
+   --  have h_lt : Exec'.lt ⟨pk.e, s', x.toNat + 1, pk.r, cr''⟩ pk := by
+   --    refine' ⟨_, _, h_prec⟩
+   --    apply Exec'.le.step _ _ _ _ h_prec'
+   --    apply Exec'.le.step _ _ _ _ h_prec''
+   --    apply Exec'.le.refl _
+   --  apply ih ⟨pk.e, s', x.toNat + 1, pk.r, cr''⟩ h_lt p h_eq hp
+
+
+  #exit
+
+
+
+
+    /-
+    rcases subcode_compile_branch sc with
+      ⟨loc, h_loc, h_push, h_jumpi, h_scp, h_jumpdest, h_scq⟩
+    have h :
+        ∃ (evm' : Evm) (ex' : Exec evm' pk.exn),
+          evm'.pc = pk.evm.pc + 3 ∧
+          Evm.Push [Nat.toB256 loc] pk.evm evm' ∧
+          Pack.Rel ⟨evm', pk.exn, ex'⟩ pk := by
+      rcases push_of_pushAt pk.ex h_push
+        with ⟨s', cr', h_pc, h, h_prec⟩
+      rw [List.toB256_pair _ h_loc] at h
+      refine' ⟨s', cr', h_pc, h, h_prec⟩
+    rcases h with ⟨s', cr, h_pc', h_push, h_prec⟩
+    rw [← h_pc'] at h_jumpi
+    simp only [Jinst.At] at h_jumpi
+    rw [h_push.code] at h_jumpi
+    rcases jumpi_at cr h_jumpi with
+        ⟨x, s'', cr', h_pc'', h_pop, h_prec'⟩
+      | ⟨x, y, s'', cr', h_pc'', h_pop, h_jmp, hy, h_prec'⟩
+    · clear h_jumpi h_scq h_jumpdest
+      have h_pop' : Evm.Pop [0] pk.evm s'' := by
+        rcases (Evm.push_cons_pop_cons h_push h_pop).right
+          with ⟨st, h_push', h_pop'⟩
+        exact rel_of_equiv_of_rel (Evm.push_nil h_push') h_pop'
+      apply Func.Run.zero h_pop'
+      have h_lt : Pack.lt ⟨s'', pk.exn, cr'⟩ pk := by
+        apply Pack.lt.intro _ h_prec
+        apply Pack.le.step _ h_prec'
+        apply Pack.le.refl _
+      rw [h_pop'.code] at eq
+      have hhh := ih ⟨s'', pk.exn, cr'⟩ h_lt p --eq
+      apply ih ⟨s'', pk.exn, cr'⟩ h_lt p tevm eq _ eq_tevm
+      simp; rw [h_pop'.code] at h_scp
+      rw [h_pc'', h_pc']; apply h_scp
+    · clear h_jumpi h_jmp h_scp
+      have h_loc' : loc < 2 ^ 256 := by
+        apply Nat.lt_trans h_loc
+        rw [Nat.pow_lt_pow_iff_right] <;> omega
+      have h : x.toNat = loc ∧ Evm.Pop [y] pk.evm s'' := by
+        rcases Evm.push_cons_pop_cons h_push h_pop
+          with ⟨hx, st, h_push', h_pop'⟩
+        constructor
+        · rw [← congrArg B256.toNat hx, toNat_toB256_of_lt h_loc']
+        · exact rel_of_equiv_of_rel (Evm.push_nil h_push') h_pop'
+      rcases h with ⟨hx, h_pop'⟩
+      have code_inv : pk.evm.code = s''.code := by
+        rw [h_push.code, h_pop.code]
+      have h_jumpdest' : Jinst.At s''.code s''.pc Jinst.jumpdest := by
+        rw [← code_inv, h_pc'', hx]; exact h_jumpdest
+      rcases jumpdest_at cr' h_jumpdest'
+        with ⟨s''', cr''', eqv, h_pc''', h_prec'''⟩
+      have h_pop_fin : Evm.Pop [y] pk.evm s''' :=
+        rel_of_rel_of_equiv h_pop' eqv
+      have h_run_fin : Func.Run (f :: fs) s''' q tevm := by
+        have eq_compile : some s'''.code.toList = Prog.compile { main := f, aux := fs } := by
+          rw [← eqv.code, ← code_inv]; exact eq
+        have subcode_q :
+            subcode s'''.code.toList s'''.pc (Func.compile (table 0 (f :: fs)) s'''.pc q) := by
+          rw [← eqv.code, ← code_inv]; rw [h_pc''', h_pc'', hx]; apply h_scq
+        have h_lt : Pack.lt { evm := s''', exn := pk.exn, ex := cr''' } pk :=
+          by apply Pack.lt.intro _ h_prec;
+             apply Pack.le.step _ h_prec';
+             apply Pack.le.step _ h_prec''';
+             apply Pack.le.refl
+        apply ih ⟨s''', pk.exn, cr'''⟩ h_lt q tevm eq_compile subcode_q eq_tevm
+      apply Func.Run.succ hy h_pop_fin h_run_fin
+      -/
+      sorry
+
+
+
+
+
+
+
+#exit
+theorem correct_core (f : Func) (fs : List Func) :
+    ∀ (pk : Pack) (p : Func),
       some pk.evm.code.toList = Prog.compile ⟨f, fs⟩ →
       subcode pk.evm.code.toList pk.evm.pc
         (Func.compile (table 0 (f :: fs)) pk.evm.pc p) →
       Func.Run (f :: fs) pk.evm p pk.exn := by
-  apply Exec'.strongRec; intro ex ih p eq sc
+  apply Pack.strongRec; intro ex ih p eq sc
   match p with
   | .last o =>
     exact Func.Run.last <| Linst.run_of_at ex.ex <| Linst.getInst_of_slice sc
@@ -445,7 +1430,7 @@ theorem correct_core (f : Func) (fs : List Func) :
       apply Ninst.getInst_of_slice; apply List.slice_prefix h_slice
     rcases Ninst.run_of_at ex.ex h_at with ⟨evm', ex', h_prec, h_pc, h_run⟩
     have h_run' : Func.Run (f :: fs) evm' p ex.exn := by
-      apply ih ⟨evm', ex.exn, ex'⟩ (Exec'.lt_of_prec h_prec) p
+      apply ih ⟨evm', ex.exn, ex'⟩ (Pack.lt_of_prec h_prec) p
       · simp; rw [← Ninst.inv_code h_run]; apply eq
       · simp; rw [h_pc, h_eq'', ← Ninst.inv_code h_run]
         apply List.slice_suffix h_slice
@@ -453,33 +1438,59 @@ theorem correct_core (f : Func) (fs : List Func) :
   | .branch p q =>
     rcases subcode_compile_branch sc with
       ⟨loc, h_loc, h_push, h_jumpi, h_scp, h_jumpdest, h_scq⟩
-      --⟨loc, h_loc, h_push, h_jumpi, h_scp, h_jumpdest, h_scq⟩
     have h :
         ∃ (evm' : Evm) (ex' : Exec evm' ex.exn),
           evm'.pc = ex.evm.pc + 3 ∧
           Evm.Push [Nat.toB256 loc] ex.evm evm' ∧
           Exec'.Rel ⟨evm', ex.exn, ex'⟩ ex := by
-      --rcases push_of_pushAt pk.cr h_push with ⟨s', cr', h, h_prec⟩
-      --rw [List.toB256_pair _ h_loc] at h
-      --refine' ⟨s', cr', h, h_prec⟩
-      sorry
+      rcases push_of_pushAt ex.ex h_push
+        with ⟨s', cr', h_pc, h, h_prec⟩
+      rw [List.toB256_pair _ h_loc] at h
+      refine' ⟨s', cr', h_pc, h, h_prec⟩
     rcases h with ⟨s', cr, h_pc', h_push, h_prec⟩
     rw [← h_pc'] at h_jumpi
     simp only [Jinst.At] at h_jumpi
     rw [h_push.code] at h_jumpi
     rcases jumpi_at cr h_jumpi with
-        ⟨x, s'', cr', h_pc', h_pop, h_prec'⟩
-      | ⟨x, y, s'', cr', h_pop, h_jmp, hy, h_prec'⟩ <;> clear h_jumpi
-    · clear h_scq h_jumpdest
+        ⟨x, s'', cr', h_pc'', h_pop, h_prec'⟩
+      | ⟨x, y, s'', cr', h_pop, h_jmp, hy, h_prec'⟩ --<;> clear h_jumpi
+    · clear h_jumpi h_scq h_jumpdest
       have h_pop' : Evm.Pop [0] ex.evm s'' := by
         rcases (Evm.push_cons_pop_cons h_push h_pop).right
           with ⟨st, h_push', h_pop'⟩
-        have foo := Evm.push_nil h_push'
+        exact rel_of_equiv_of_rel (Evm.push_nil h_push') h_pop'
+      apply Func.Run.zero h_pop'
+      have h_lt : Exec'.lt ⟨s'', ex.exn, cr'⟩ ex := by
+        apply Exec'.lt.intro _ h_prec
+        apply Exec'.le.step _ _ _ _ h_prec'
+        apply Exec'.le.refl _
+      rw [h_pop'.code] at eq
+      apply ih ⟨s'', ex.exn, cr'⟩ h_lt p eq
+      simp; rw [h_pop'.code] at h_scp
+      rw [h_pc'', h_pc']; apply h_scp
+    · clear h_jumpi h_jmp h_scp
+      have h_loc' : loc < 2 ^ 256 := by
+        apply Nat.lt_trans h_loc
+        rw [Nat.pow_lt_pow_iff_right] <;> omega
+      have h : x.toNat = loc ∧ Evm.Pop [y] ex.evm s'' := by
+        rcases Evm.push_cons_pop_cons h_push h_pop
+          with ⟨hx, st, h_push', h_pop'⟩
+        constructor
+        · rw [← congrArg B256.toNat hx, toNat_toB256_of_lt h_loc']
+        · exact rel_of_equiv_of_rel (Evm.push_nil h_push') h_pop'
+      rcases h with ⟨hx, h_pop'⟩
+      have h_run' : Func.Run (f :: fs) s'' q ex.exn := by
+        rw [← hx] at h_jumpdest
+        rcases jumpdest_at cr' h_jumpdest with ⟨cr'', h_prec''⟩
 
-        -- rw [Desc.push_nil h_push']; exact h_pop'
-      -- apply Func.Run.zero h_pop'
-      -- have h_lt : Exec'.lt ⟨pk.e, s'', pk.pc +4, pk.r, cr'⟩ pk := by
-      --   refine' ⟨_, _, h_prec⟩
-      --   apply Exec'.le.step _ _ _ _ h_prec'
-      --   apply Exec'.le.refl _
-      -- apply ih ⟨pk.e, s'', pk.pc + 4, pk.r, cr'⟩ h_lt p h_eq h_scp
+      #exit
+        rw [← hx] at h_jumpdest
+        rcases jumpdest_at cr' h_jumpdest with ⟨cr'', h_prec''⟩
+        have h_lt : Exec'.lt ⟨pk.e, s'', x.toNat + 1, pk.r, cr''⟩ pk := by
+          refine' ⟨_, _, h_prec⟩
+          apply Exec'.le.step _ _ _ _ h_prec'
+          apply Exec'.le.step _ _ _ _ h_prec''
+          apply Exec'.le.refl _
+        rw [← hx] at h_scq
+        apply ih ⟨pk.e, s'', x.toNat + 1, pk.r, cr''⟩ h_lt q h_eq h_scq
+      apply Func.Run.succ hy h_pop' h_run'
